PolyFun.lean
@@ -161,11 +161,11 @@ import PolyFun.PFunctor.Dynamical.Responder.Parallel.Behavior
 import PolyFun.PFunctor.Dynamical.Responder.Parallel.Coherence
 import PolyFun.PFunctor.Dynamical.Responder.Parallel.Compatibility
 import PolyFun.PFunctor.Dynamical.Responder.Parallel.Display
-import PolyFun.PFunctor.Dynamical.Responder.Parallel.VerifiedAssociativity
-import PolyFun.PFunctor.Dynamical.Responder.Parallel.VerifiedCoherence
-import PolyFun.PFunctor.Dynamical.Responder.Parallel.VerifiedPresentation
+import PolyFun.PFunctor.Dynamical.Responder.Parallel.DisplayedAssociativity
+import PolyFun.PFunctor.Dynamical.Responder.Parallel.DisplayedCoherence
+import PolyFun.PFunctor.Dynamical.Responder.Parallel.Presentation
+import PolyFun.PFunctor.Dynamical.Responder.Presentation
 import PolyFun.PFunctor.Dynamical.Responder.Reindex
-import PolyFun.PFunctor.Dynamical.Responder.VerifiedPresentation
 import PolyFun.PFunctor.Dynamical.Run
 import PolyFun.PFunctor.Dynamical.RunN
 import PolyFun.PFunctor.Dynamical.Safety
